Removing CircuitLib.

CircuitBounds.dfy
@@ -5,148 +5,98 @@ module CircuitBounds {
     import opened Circuit
     import Seq=Std.Collections.Seq
 
-    function GetSubCRef(lib: CLib, c: Circuit, n: CNode): (r: Option<CircuitRef>)
-        requires CircuitValid(lib, c)
-        ensures r.None? || (CRefCircuitValid(lib, r.value) && CRefHierLevelReduced(lib, c, r.value))
-        ensures c.NodeKind(n).Some? && c.NodeKind(n).value.CHier? ==>
-            r.Some? && (r.value == c.NodeKind(n).value.CRef)
-    {
-        reveal CircuitValid();
-        assert CircuitNodeKindValid(lib, c);
-        match c.NodeKind(n)
-            case Some(nk) => (
-                match nk
-                case CHier(cref) =>
-                    assert CNodeKindValid(lib, c.HierLevel, c.PortBound, nk);
-                    assert CRefValid(lib, cref);
-                    Some(cref)
-                case _ => None
-            )
-            case _ => None
-    }
-
-    predicate CRefHierLevelReduced(lib: CLib, c: Circuit, cref: CircuitRef)
-        requires CircuitValid(lib, c)
-        requires CRefCircuitValid(lib, cref)
-    {
-        var unref_c := lib.Circuits[cref];
-        unref_c.HierLevel < c.HierLevel
-    }
-
-    function DirectSubCRefsInternal(lib: CLib, c: Circuit, n: CNode, subcircuits: seq<CircuitRef>): (r: seq<CircuitRef>)
-        requires CircuitValid(lib, c)
-        requires forall i: nat :: i < |subcircuits| ==>
-            CRefCircuitValid(lib, subcircuits[i]) && CRefHierLevelReduced(lib, c, subcircuits[i])
-        requires forall m: CNode :: m >= n && c.NodeKind(m).Some? && c.NodeKind(m).value.CHier? ==> c.NodeKind(m).value.CRef in subcircuits
-        ensures forall i: nat :: i < |r| ==>
-            CRefCircuitValid(lib, r[i]) && CRefHierLevelReduced(lib, c, r[i])
-        ensures forall m: CNode :: c.NodeKind(m).Some? && c.NodeKind(m).value.CHier? ==>
-            c.NodeKind(m).value.CRef in r
-    {
-        if n == 0 then
-            subcircuits
-        else
-            var new_cref := GetSubCRef(lib, c, n-1);
-            var updated_subcircuits: seq<CircuitRef> :=
-                match new_cref
-                    case Some(cref) => subcircuits + [cref]
-                    case None => subcircuits;
-            DirectSubCRefsInternal(lib, c, n-1, updated_subcircuits)
-    }
-
-    function DirectSubCRefs(lib: CLib, c: Circuit): (r: seq<CircuitRef>)
-        requires CircuitValid(lib, c)
-        ensures forall m: CNode :: c.NodeKind(m).Some? && c.NodeKind(m).value.CHier? ==>
-            c.NodeKind(m).value.CRef in r
-        ensures forall cref: CircuitRef :: cref in r ==>
-            CRefCircuitValid(lib, cref) && CRefHierLevelReduced(lib, c, cref)
-    {
-        reveal CircuitValid();
-        assert CircuitNodeKindValid(lib, c);
-        assert forall n: CNode :: n >= c.NodeBound ==> c.NodeKind(n).None?;
-        DirectSubCRefsInternal(lib, c, c.NodeBound, [])
-    }
-
     lemma {:vcs_split_on_every_assert} HierBoundEncloses(
-            lib: CLib, c: Circuit, bound_f: Circuit -> nat, hp: HierarchyPath)
-        requires CircuitValid(lib, c)
-        requires HierarchyPathValid(lib, c, hp)
+            c: Circuit, bound_f: Circuit -> nat, hp: HierarchyPath)
+        requires CircuitValid(c)
+        requires HierarchyPathValid(c, hp)
         ensures
-            var hierc := HierarchyPathCircuit(lib, c, hp);
-            CircuitValid(lib, hierc) &&
-            HierBound(lib, hierc, bound_f) <= HierBound(lib, c, bound_f)
+            var hierc := HierarchyPathCircuit(c, hp);
+            CircuitValid(hierc) &&
+            HierBound(hierc, bound_f) <= HierBound(c, bound_f)
         decreases |hp.v|
     {
-        var hierc := HierarchyPathCircuit(lib, c, hp);
-        HierarchyPathCircuitValid(lib, c, hp);
+        var hierc := HierarchyPathCircuit(c, hp);
+        HierarchyPathCircuitValid(c, hp);
         if |hp.v| == 0 {
-            assert HierBound(lib, hierc, bound_f) <= HierBound(lib, c, bound_f);
+            assert HierBound(hierc, bound_f) <= HierBound(c, bound_f);
         } else {
             var (head, tail) := HPHeadTail(hp);
-            HierBoundEncloses(lib, c, bound_f, tail);
-            var tail_c := HierarchyPathCircuit(lib, c, tail);
-            HierarchyPathCircuitValid(lib, c, tail);
-            assert HierBound(lib, tail_c, bound_f) <= HierBound(lib, c, bound_f);
-            assert HierBound(lib, hierc, bound_f) <= HierBound(lib, c, bound_f);
+            HierBoundEncloses(c, bound_f, tail);
+            var tail_c := HierarchyPathCircuit(c, tail);
+            HierarchyPathCircuitValid(c, tail);
+            assert HierBound(tail_c, bound_f) <= HierBound(c, bound_f);
+            assert HierBound(hierc, bound_f) <= HierBound(c, bound_f);
         }
     }
 
-    function GetSubBounds(lib: CLib, c: Circuit, bound_f: Circuit -> nat): (r: seq<nat>)
-        requires CircuitValid(lib, c)
+    lemma GetSubBoundsHelper(c: Circuit)
+        requires CircuitValid(c)
         ensures forall m: CNode :: c.NodeKind(m).Some? && c.NodeKind(m).value.CHier? ==>
-            CRefValid(lib, c.NodeKind(m).value.CRef) &&
-            var subc := lib.Circuits[c.NodeKind(m).value.CRef];
-            CircuitValid(lib, subc) &&
+            var subc := c.NodeKind(m).value.c;
+            subc in DirectSubcircuits(c)
+    {
+        forall m: CNode | c.NodeKind(m).Some? && c.NodeKind(m).value.CHier?
+            ensures
+                var subc := c.NodeKind(m).value.c;
+                subc in DirectSubcircuits(c)
+        {
+            SubcircuitInDirectSubcircuits(c, m);
+        }
+
+    }
+
+    function GetSubBounds(c: Circuit, bound_f: Circuit -> nat): (r: seq<nat>)
+        requires CircuitValid(c)
+        ensures forall m: CNode :: c.NodeKind(m).Some? && c.NodeKind(m).value.CHier? ==>
+            var subc := c.NodeKind(m).value.c;
+            CircuitValid(subc) &&
             subc.HierLevel < c.HierLevel &&
-            HierBound(lib, subc, bound_f) in r
+            HierBound(subc, bound_f) in r
         decreases c.HierLevel, 0
     {
-        var subcrefs := DirectSubCRefs(lib, c);
+        var subcs: seq<Circuit> := DirectSubcircuits(c);
         var new_bound := bound_f(c);
-        assert forall m: CNode :: c.NodeKind(m).Some? && c.NodeKind(m).value.CHier? ==>
-            var subcref := c.NodeKind(m).value.CRef;
-            subcref in subcrefs;
+        AllSubcircuitsValid(c);
         var bounds := Seq.Map(
-            cref requires CRefCircuitValid(lib, cref) && CRefHierLevelReduced(lib, c, cref)  =>
-                HierBound(lib, lib.Circuits[cref], bound_f),
-            subcrefs);
+            subc requires CircuitValid(subc) && (subc.HierLevel < c.HierLevel)  =>
+                HierBound(subc, bound_f),
+            subcs);
+        GetSubBoundsHelper(c);
         assert forall m: CNode :: c.NodeKind(m).Some? && c.NodeKind(m).value.CHier? ==>
-            var subcref := c.NodeKind(m).value.CRef;
-            var subc := lib.Circuits[subcref];
-            var index: nat :| index < |subcrefs| && subcrefs[index] == subcref;
-            (bounds[index] == HierBound(lib, subc, bound_f)) &&
-            (HierBound(lib, subc, bound_f) in bounds);
+            var subc := c.NodeKind(m).value.c;
+            assert subc in subcs;
+            var index: nat :| index < |subcs| && subcs[index] == subc;
+            (bounds[index] == HierBound(subc, bound_f)) &&
+            (HierBound(subc, bound_f) in bounds);
         bounds
     }
 
-    function {:vcs_split_on_every_assert} HierBound(lib: CLib, c: Circuit, bound_f: Circuit -> nat): (r: nat)
-        requires CircuitValid(lib, c)
+    function {:vcs_split_on_every_assert} HierBound(c: Circuit, bound_f: Circuit -> nat): (r: nat)
+        requires CircuitValid(c)
         ensures forall m: CNode :: c.NodeKind(m).Some? && c.NodeKind(m).value.CHier? ==>
-            CRefValid(lib, c.NodeKind(m).value.CRef) &&
-            var subc := lib.Circuits[c.NodeKind(m).value.CRef];
-            CircuitValid(lib, subc) &&
+            var subc := c.NodeKind(m).value.c;
+            CircuitValid(subc) &&
             subc.HierLevel < c.HierLevel &&
-            HierBound(lib, subc, bound_f) <= r
+            HierBound(subc, bound_f) <= r
         ensures bound_f(c) as nat <= r
         decreases c.HierLevel, 1
     {
-        var bounds := GetSubBounds(lib, c, bound_f);
+        var bounds := GetSubBounds(c, bound_f);
         var new_bound := bound_f(c);
         var combined_bounds := bounds + [new_bound];
         var max_bound := Seq.Max(combined_bounds);
         assert new_bound in combined_bounds;
         assert new_bound <= max_bound;
-        var subcrefs := DirectSubCRefs(lib, c);
+        var subcircuits := DirectSubcircuits(c);
         assert forall pb: nat :: pb in bounds+[new_bound] ==> pb <= max_bound;
+        GetSubBoundsHelper(c);
         assert forall m: CNode :: c.NodeKind(m).Some? && c.NodeKind(m).value.CHier? ==>
-            var subcref := c.NodeKind(m).value.CRef;
-            (subcref in subcrefs) && 
-            var subc := lib.Circuits[subcref];
-            (HierBound(lib, subc, bound_f) in bounds + [bound_f(c)]);
+            var subc := c.NodeKind(m).value.c;
+            (subc in subcircuits) && 
+            (HierBound(subc, bound_f) in bounds + [new_bound]);
         assert forall m: CNode :: c.NodeKind(m).Some? && c.NodeKind(m).value.CHier? ==>
-            var subcref := c.NodeKind(m).value.CRef;
-            var subc := lib.Circuits[subcref];
-            (HierBound(lib, subc, bound_f) <= max_bound);
+            var subc := c.NodeKind(m).value.c;
+            (HierBound(subc, bound_f) <= max_bound);
         max_bound
     }
 
@@ -168,107 +118,106 @@ module CircuitBounds {
         c.NodeBound as nat
     }
 
-    function HierPortBound(lib: CLib, c: Circuit): nat
-        requires CircuitValid(lib, c)
+    function HierPortBound(c: Circuit): nat
+        requires CircuitValid(c)
     {
-        HierBound(lib, c, getpb)
+        HierBound(c, getpb)
     }
 
-    function HierNodeBound(lib: CLib, c: Circuit): nat
-        requires CircuitValid(lib, c)
+    function HierNodeBound(c: Circuit): nat
+        requires CircuitValid(c)
     {
-        HierBound(lib, c, getnb)
+        HierBound(c, getnb)
     }
 
-    lemma SubcircuitInHierPortBound(lib: CLib, c: Circuit, hp: HierarchyPath)
-        requires CircuitValid(lib, c)
-        requires HierarchyPathValid(lib, c, hp)
+    lemma SubcircuitInHierPortBound(c: Circuit, hp: HierarchyPath)
+        requires CircuitValid(c)
+        requires HierarchyPathValid(c, hp)
         ensures
-            var hier_c := HierarchyPathCircuit(lib, c, hp);
-            hier_c.PortBound as nat <= HierPortBound(lib, c)
+            var hier_c := HierarchyPathCircuit(c, hp);
+            hier_c.PortBound as nat <= HierPortBound(c)
     {
-        HierBoundEncloses(lib, c, getpb, hp);
+        HierBoundEncloses(c, getpb, hp);
     }
 
 
-    lemma SubcircuitInHierNodeBound(lib: CLib, c: Circuit, hp: HierarchyPath)
-        requires CircuitValid(lib, c)
-        requires HierarchyPathValid(lib, c, hp)
+    lemma SubcircuitInHierNodeBound(c: Circuit, hp: HierarchyPath)
+        requires CircuitValid(c)
+        requires HierarchyPathValid(c, hp)
         ensures
-            var hier_c := HierarchyPathCircuit(lib, c, hp);
-            hier_c.NodeBound as nat <= HierNodeBound(lib, c)
+            var hier_c := HierarchyPathCircuit(c, hp);
+            hier_c.NodeBound as nat <= HierNodeBound(c)
     {
-        HierBoundEncloses(lib, c, getnb, hp);
+        HierBoundEncloses(c, getnb, hp);
     }
 
-    lemma HPInHierNodeBound(lib: CLib, c: Circuit, hp: HierarchyPath)
-        requires CircuitValid(lib, c)
-        requires HierarchyPathValid(lib, c, hp)
+    lemma HPInHierNodeBound(c: Circuit, hp: HierarchyPath)
+        requires CircuitValid(c)
+        requires HierarchyPathValid(c, hp)
         ensures
-            forall n: CNode :: (n in hp.v) ==> n as nat < HierNodeBound(lib, c)
+            forall n: CNode :: (n in hp.v) ==> n as nat < HierNodeBound(c)
         decreases |hp.v|
     {
         if |hp.v| == 0 {
         } else {
             var (head, tail) := HPHeadTail(hp);
-            var hier_c := HierarchyPathCircuit(lib, c, hp);
-            var tail_c := HierarchyPathCircuit(lib, c, tail);
-            HierarchyPathCircuitValid(lib, c, tail);
+            var hier_c := HierarchyPathCircuit(c, hp);
+            var tail_c := HierarchyPathCircuit(c, tail);
+            HierarchyPathCircuitValid(c, tail);
             reveal CircuitValid();
             assert head <= tail_c.NodeBound;
-            SubcircuitInHierNodeBound(lib, c, tail);
-            assert tail_c.NodeBound as nat <= HierNodeBound(lib, c);
-            HPInHierNodeBound(lib, c, tail);
-            assert head as nat <= HierNodeBound(lib, c);
-            assert forall n: CNode :: (n in tail.v) ==> n as nat < HierNodeBound(lib, c);
-            assert forall n: CNode :: (n in tail.v + [head]) ==> n as nat < HierNodeBound(lib, c);
+            SubcircuitInHierNodeBound(c, tail);
+            assert tail_c.NodeBound as nat <= HierNodeBound(c);
+            HPInHierNodeBound(c, tail);
+            assert head as nat <= HierNodeBound(c);
+            assert forall n: CNode :: (n in tail.v) ==> n as nat < HierNodeBound(c);
+            assert forall n: CNode :: (n in tail.v + [head]) ==> n as nat < HierNodeBound(c);
             assert tail.v + [head] == hp.v;
         }
     }
 
     // Show that the any valid hpnp is smaller than total bound
 
-    function HPNPElementBound(lib: CLib, c: Circuit): nat
-        requires CircuitValid(lib, c)
+    function HPNPElementBound(c: Circuit): nat
+        requires CircuitValid(c)
     {
-        var max_node_index := HierNodeBound(lib, c);
-        var max_port_index := HierPortBound(lib, c);
+        var max_node_index := HierNodeBound(c);
+        var max_port_index := HierPortBound(c);
         var max_index := if max_node_index > max_port_index then max_node_index else max_port_index;
         max_index
     }
 
-    lemma HPNPElementsInBound(lib: CLib, c: Circuit, hpnp: HPNP)
-        requires CircuitValid(lib, c)
-        requires HPNPValid(lib, c, hpnp)
+    lemma HPNPElementsInBound(c: Circuit, hpnp: HPNP)
+        requires CircuitValid(c)
+        requires HPNPValid(c, hpnp)
         ensures
-            forall n: CNode :: (n in hpnp.hpn.hp.v) ==> n as nat < HPNPElementBound(lib, c)
-        ensures hpnp.hpn.n as nat < HPNPElementBound(lib, c)
-        ensures hpnp.p as nat < HPNPElementBound(lib, c)
+            forall n: CNode :: (n in hpnp.hpn.hp.v) ==> n as nat < HPNPElementBound(c)
+        ensures hpnp.hpn.n as nat < HPNPElementBound(c)
+        ensures hpnp.p as nat < HPNPElementBound(c)
     {
-        var element_bound := HPNPElementBound(lib, c);
-        HPNPValidHPValid(lib, c, hpnp);
-        HPInHierNodeBound(lib, c, hpnp.hpn.hp);
-        var hier_c := HierarchyPathCircuit(lib, c, hpnp.hpn.hp);
-        HierarchyPathCircuitValid(lib, c, hpnp.hpn.hp);
-        SubcircuitInHierNodeBound(lib, c, hpnp.hpn.hp);
+        var element_bound := HPNPElementBound(c);
+        HPNPValidHPValid(c, hpnp);
+        HPInHierNodeBound(c, hpnp.hpn.hp);
+        var hier_c := HierarchyPathCircuit(c, hpnp.hpn.hp);
+        HierarchyPathCircuitValid(c, hpnp.hpn.hp);
+        SubcircuitInHierNodeBound(c, hpnp.hpn.hp);
         assert hier_c.NodeBound as nat <= element_bound;
-        SubcircuitInHierPortBound(lib, c, hpnp.hpn.hp);
+        SubcircuitInHierPortBound(c, hpnp.hpn.hp);
         assert hier_c.PortBound as nat <= element_bound;
         reveal CircuitValid();
-        assert CircuitNodeKindValid(lib, hier_c);
+        assert CircuitNodeKindValid(hier_c);
         reveal HPNPValidInput();
         reveal HPNPValidOutput();
         assert hpnp.p < hier_c.PortBound;
         assert hpnp.hpn.n < hier_c.NodeBound;
     }
 
-    function HPNPBound(lib: CLib, c: Circuit): nat
-        requires CircuitValid(lib, c)
+    function HPNPBound(c: Circuit): nat
+        requires CircuitValid(c)
     {
-        var max_index := HPNPElementBound(lib, c);
+        var max_index := HPNPElementBound(c);
         var ns := Seq.Repeat(max_index, c.HierLevel+2);
         SeqNatToNat.ArbLenNatsToNat(ns)
     }
-
 
 }
