SeqExt.dfy
@@ -16,4 +16,21 @@ module SeqExt {
     {
         reveal Seq.HasNoDuplicates();
     }
+
+    lemma FilterStillContains<X>(f: X -> bool, xs: seq<X>, x: X)
+        requires f(x)
+        requires x in xs
+        ensures x in Seq.Filter(f, xs)
+    {
+        reveal Seq.Filter();
+    }
+
+    lemma MapStillContains<X, Y>(f: X --> Y, xs: seq<X>, x: X)
+        requires x in xs
+        requires f.requires(x)
+        requires forall xx :: xx in xs ==> f.requires(xx)
+        ensures f(x) in Seq.Map(f, xs)
+    {
+        reveal Seq.Map();
+    }
 }
